thys/Abstract_Monitor.thy
@@ -154,7 +154,7 @@ fun past_only :: "Formula.formula \<Rightarrow> bool" where
 | "past_only (Formula.And \<alpha> \<beta>) = (past_only \<alpha> \<and> past_only \<beta>)"
 | "past_only (Formula.Ands l) = (\<forall>\<alpha>\<in>set l. past_only \<alpha>)"
 | "past_only (Formula.Exists \<psi>) = past_only \<psi>"
-| "past_only (Formula.Agg _ _ _ _ _ \<psi>) = past_only \<psi>"
+| "past_only (Formula.Agg _ _ _ _ \<psi>) = past_only \<psi>"
 | "past_only (Formula.Prev _ \<psi>) = past_only \<psi>"
 | "past_only (Formula.Next _ _) = False"
 | "past_only (Formula.Since \<alpha> _ \<beta>) = (past_only \<alpha> \<and> past_only \<beta>)"
